Simplify both mover proof.

ironfleet/src/Dafny/Distributed/Services/Lock/AtomicTrace.i.dfy
@@ -137,62 +137,51 @@ module AtomicTrace_i {
                     .(servers := qb3.servers);
     }
 
+    predicate ComputeStep(qb:QS_State, qb':QS_State)
+    {
+        var step  := qb.environment.nextStep;
+        var step' := qb'.environment.nextStep;
+                     step.LEnvStepHostIos? 
+                  && step.actor in qb.servers    // It's one of our hosts
+                  && |step.ios| == 0
+                  && (step'.LEnvStepHostIos? ==> step'.actor != step.actor) // Other step wasn't this host
+    }
 
-//                  X        C      
-//    qb0 ---> qb1 ---> qb2 ---> qb3 
-//              \               /
-//           C   \             /  X
-//                > qb2' ---->
-    lemma HostComputeIsALeftMover(qb0:QS_State, qb1:QS_State, qb2:QS_State, qb3:QS_State) returns (qb1':QS_State, qb2':QS_State)
+    lemma HostComputeIsABothMover(qb0:QS_State, qb1:QS_State, qb2:QS_State, qb3:QS_State) returns (qb1':QS_State, qb2':QS_State)
         requires QS_Next(qb0, qb1);
         requires QS_Next(qb1, qb2);
         requires QS_Next(qb2, qb3);
-        requires var step := qb2.environment.nextStep;
-                    step.LEnvStepHostIos? 
-                 && step.actor in qb2.servers    // It's one of our hosts
-                 && |step.ios| == 0;
-        requires var step := qb1.environment.nextStep;      // Previous step wasn't this host
-                    step.LEnvStepHostIos? ==> step.actor != qb2.environment.nextStep.actor;
+        requires ComputeStep(qb1, qb2) || ComputeStep(qb2, qb1);
         ensures  QS_Next(qb0, qb1');
         ensures  QS_Next(qb1', qb2');
         ensures  QS_Next(qb2', qb3);
         ensures  qb1' == qb1.(environment := qb1.environment.(nextStep := qb2.environment.nextStep));
         ensures  qb2'.environment.nextStep == qb1.environment.nextStep;
     {
-        var host := qb2.environment.nextStep.actor;
-        qb1' := qb1.(environment := qb1.environment.(nextStep := qb2.environment.nextStep));
-        qb2' := qb1'.(environment := qb1.environment.(nextStep := qb1.environment.nextStep))
-                   .(servers := qb1.servers[host := qb3.servers[host]]);
+        if ComputeStep(qb1, qb2) {
+            //                  C        X      
+            //    qb0 ---> qb1 ---> qb2 ---> qb3 
+            //              \               /
+            //           X   \             /  C
+            //                > qb2' ---->
+
+            var host := qb1.environment.nextStep.actor;
+            qb1' := qb1.(environment := qb1.environment.(nextStep := qb2.environment.nextStep));
+            qb2' := qb1'.(environment := qb3.environment.(nextStep := qb1.environment.nextStep))
+                        .(servers := qb3.servers[host := qb1.servers[host]]);
+        } else {
+            //                  X        C      
+            //    qb0 ---> qb1 ---> qb2 ---> qb3 
+            //              \               /
+            //           C   \             /  X
+            //                > qb2' ---->
+            var host := qb2.environment.nextStep.actor;
+            qb1' := qb1.(environment := qb1.environment.(nextStep := qb2.environment.nextStep));
+            qb2' := qb1'.(environment := qb1.environment.(nextStep := qb1.environment.nextStep))
+                       .(servers := qb1.servers[host := qb3.servers[host]]);
+        }
     }
 
-
-
-//                  C        X      
-//    qb0 ---> qb1 ---> qb2 ---> qb3 
-//              \               /
-//           X   \             /  C
-//                > qb2' ---->
-    lemma HostComputeIsARightMover(qb0:QS_State, qb1:QS_State, qb2:QS_State, qb3:QS_State) returns (qb1':QS_State, qb2':QS_State)
-        requires QS_Next(qb0, qb1);
-        requires QS_Next(qb1, qb2);
-        requires QS_Next(qb2, qb3);
-        requires var step := qb1.environment.nextStep;
-                    step.LEnvStepHostIos? 
-                 && step.actor in qb1.servers    // It's one of our hosts
-                 && |step.ios| == 0;
-        requires var step := qb2.environment.nextStep;      // Next step isn't this host
-                    step.LEnvStepHostIos? ==> step.actor != qb1.environment.nextStep.actor;
-        ensures  QS_Next(qb0, qb1');
-        ensures  QS_Next(qb1', qb2');
-        ensures  QS_Next(qb2', qb3);
-        ensures  qb1' == qb1.(environment := qb1.environment.(nextStep := qb2.environment.nextStep));
-        ensures  qb2'.environment.nextStep == qb1.environment.nextStep;
-    {
-        var host := qb1.environment.nextStep.actor;
-        qb1' := qb1.(environment := qb1.environment.(nextStep := qb2.environment.nextStep));
-        qb2' := qb1'.(environment := qb3.environment.(nextStep := qb1.environment.nextStep))
-                    .(servers := qb3.servers[host := qb1.servers[host]]);
-    }
 
 // TODO: Maybe we don't need ConcreteConfiguration
     ghost method MakeAtomicTrace(config:ConcreteConfiguration, qb:seq<QS_State>, external_io:SpecIoFilter) returns (qb':seq<QS_State>, db':seq<DS_State>) //, cm:seq<int>)
